src/functional/TreeSort.dfy
@@ -1,73 +1,40 @@
 include "./BST.dfy"
 include "./List.dfy"
 
-function method TreeSort(list:List<int>, tree:BST<T>) : (sortedList:List<int>)
-  // Lemma_TreeSortListIsOrdered(list, tree) ==> ensures list_is_ordered(TreeSort(list, Leaf))
+function method TreeSort(list:List<int>) : (sortedList:List<int>)
+  // Lemma_TreeSortListIsOrdered(list) ==> ensures list_is_ordered(TreeSort(list))
+  // Lemma_TreeSortSameElemsThanList ==> ensures List_ToMultiset(TreeSort(list)) == List_ToMultiset(list)
   decreases list
 {
-  match list {
-    case Cons(head, tail) => TreeSort(tail, BST_Insert(tree, head))
-    case List_Empty => BST_InOrder(tree)
+  BST_InOrder(BST_Load(list))
+}
+
+lemma {:induction list} Lemma_TreeSortListIsOrdered(list:List<T>)
+  ensures list_is_ordered(TreeSort(list))
+{
+  calc == {
+    list_is_ordered(TreeSort(list));
+      { assert TreeSort(list) == BST_InOrder(BST_Load(list)); }
+    list_is_ordered(BST_InOrder(BST_Load(list)));
+      { Lemma_LoadIsOrdered(list); }
+      { assert bst_is_ordered(BST_Load(list)); }
+      { Lemma_BSTOrderedThenInOrderOrdered(BST_Load(list)); }
+    true;
   }
 }
 
-/*
-lemma {:induction list} Lemma_TreeSortListIsOrdered(list:List<T>, tree:BST<T>)
-  ensures list_is_ordered(TreeSort(list, tree))
+lemma {:induction list} Lemma_TreeSortSameElemsThanList(list:List<T>)
+  ensures List_ToMultiset(TreeSort(list)) == List_ToMultiset(list)
 {
-  match list {
-    case List_Empty =>
-      calc == {
-        list_is_ordered(TreeSort(list, Leaf));
-          { assert list == List_Empty; }
-        list_is_ordered(TreeSort(List_Empty, Leaf));
-          { assert TreeSort(List_Empty, Leaf) == BST_InOrder(Leaf); }
-        list_is_ordered(BST_InOrder(Leaf));
-          { assert BST_InOrder(Leaf) == List_Empty; }
-        list_is_ordered(List_Empty);
-          { assert list_is_ordered(List_Empty) == true; }
-        true;
-      }
-    case Cons(head, tail) =>
-      calc == {
-        list_is_ordered(TreeSort(list, Leaf));
-          { assert list == Cons(head, tail); }
-        list_is_ordered(TreeSort(Cons(head, tail), Leaf));
-          { assert TreeSort(Cons(head, tail), Leaf) == TreeSort(tail, BST_Insert(Leaf, head)); }
-        list_is_ordered(TreeSort(tail, BST_Insert(Leaf, head)));
-          { Lemma_InsertOrdered(tree, head); }
-          { assert BST_Insert(Leaf, head) == Node(Leaf, head, Leaf); }
-        list_is_ordered(TreeSort(tail, Node(Leaf, head, Leaf)));
-        match tail {
-          case List_Empty =>
-            calc == {
-              list_is_ordered(TreeSort(tail, Node(Leaf, head, Leaf)));
-                { assert tail == List_Empty; }
-              list_is_ordered(TreeSort(List_Empty, Node(Leaf, head, Leaf)));
-                { assert TreeSort(List_Empty, Node(Leaf, head, Leaf)) == BST_InOrder(Node(Leaf, head, Leaf)); }
-              list_is_ordered(BST_InOrder(Node(Leaf, head, Leaf)));
-                { assert BST_InOrder(Node(Leaf, head, Leaf)) == List_Concat(BST_InOrder(Leaf), Cons(head, BST_InOrder(Leaf))); }
-              list_is_ordered(List_Concat(BST_InOrder(Leaf), Cons(head, BST_InOrder(Leaf))));
-                { assert BST_InOrder(Leaf) == List_Empty; }
-              list_is_ordered(List_Concat(List_Empty, Cons(head, List_Empty)));
-                { Lemma_ConcatFirstListEmpty(List_Empty, Cons(head, List_Empty)); }
-              list_is_ordered(Cons(head, List_Empty));
-                { assert list_is_ordered(Cons(head, List_Empty)) == true; }
-              true;
-            }
-          case Cons(tah, tat) =>
-            calc == {
-              list_is_ordered(TreeSort(tail, Node(Leaf, head, Leaf)));
-                { assert tail == Cons(tah, tat); }
-              list_is_ordered(TreeSort(Cons(tah, tat), Node(Leaf, head, Leaf)));
-                { assert TreeSort(Cons(tah, tat), Node(Leaf, head, Leaf)) == TreeSort(tat, BST_Insert(Node(Leaf, head, Leaf), tah)); }
-              list_is_ordered(TreeSort(tat, BST_Insert(Node(Leaf, head, Leaf), tah)));
-                { Lemma_TreeSortListIsOrdered(tat, BST_Insert(Node(Leaf, head, Leaf), tah)); }
-              true;
-            }
-        }
-        true;
-      }
+  calc == {
+    List_ToMultiset(TreeSort(list));
+      { assert TreeSort(list) == BST_InOrder(BST_Load(list)); }
+    List_ToMultiset(BST_InOrder(BST_Load(list)));
+      { Lemma_LoadIsOrdered(list); }
+      { assert bst_is_ordered(BST_Load(list)); }
+      { Lemma_BSTSameElementsThanInOrder(BST_Load(list)); }
+    BST_ToMultiset(BST_Load(list));
+      { Lemma_LoadTreeElemsSameThanList(list); }
+    List_ToMultiset(list);
   }
 }
-*/
