test/functional/TreeSortTest.dfy
@@ -1,11 +1,26 @@
 include "../../src/functional/TreeSort.dfy"
 
 method Main() {
-  TreeSortTest();
+  Test_TreeSort();
+  Test_Lemma_TreeSortListIsOrdered();
+  Test_Lemma_TreeSortSameElemsThanList();
 }
 
-method TreeSortTest() {
+method Test_TreeSort() {
   var list := Cons(2, Cons(10, Cons(4, Cons(12, Cons(7, List_Empty)))));
-  var sorted := TreeSort(list, Leaf);
-  List_Print(sorted);
+  var sorted := TreeSort(list);
+  var expected := Cons(2, Cons(4, Cons(7, Cons(10, Cons(12, List_Empty)))));
+  assert expected == sorted;
+}
+
+method Test_Lemma_TreeSortListIsOrdered() {
+  var list := Cons(2, Cons(10, Cons(4, Cons(12, Cons(7, List_Empty)))));
+  { Lemma_TreeSortListIsOrdered(list); }
+  assert list_is_ordered(TreeSort(list));
+}
+
+method Test_Lemma_TreeSortSameElemsThanList() {
+  var list := Cons(2, Cons(10, Cons(4, Cons(12, Cons(7, List_Empty)))));
+  { Lemma_TreeSortSameElemsThanList(list); }
+  assert List_ToMultiset(TreeSort(list)) == List_ToMultiset(list);
 }
